continuity lemma

src/multiplier.v
@@ -1,6 +1,6 @@
 (**********************************************************************************)
 (*                                                                                *)
-(*  multiplier.v - Shift-and-add 4-bit multiplier.                                *)
+(*             multiplier.v - Shift-and-add 4-bit multiplier.                     *)
 (*                                                                                *)
 (*                   +---------------------------+                                *)
 (*                   |                           |                                *)
@@ -13,8 +13,8 @@
 (*                   +---------------------------+                                *)
 (*                                                                                *)
 (*  The main theorem is a statement of a cryptographic constant-time (CCT)        *)
-(*  hyperproperty. The statement of the property looks as follows (which we state *)
-(*  as an equivalent single-copy trace property):                                 *)
+(*  hyperproperty. The statement of the property looks as follows (which we       *)
+(*  state as an equivalent single-copy trace property):                           *)
 (*                                                                                *)
 (*  There exists some predictor [f] such that given a cycle schedule [C],         *)
 (*  starting from a reset state, the multiplier circuit [M] will produce an       *)
@@ -23,11 +23,11 @@
 (*  A specification leakage trace [t] is extracted from schedule [C] which        *)
 (*  will record the values of [A] and [valid] each cycle. On termination,         *)
 (*                                                                                *)
-(*                              [t' = f(t)].                                      *)
+(*                              [t' = f t].                                       *)
 (*                                                                                *)
 (**********************************************************************************)
 
-From stdpp Require Import base tactics bitvector.
+From stdpp Require Import base tactics bitvector list.
 From RecordUpdate Require Import RecordUpdate.
 
 Local Open Scope bv_scope.
@@ -44,7 +44,7 @@ Tactic Notation "unfold" "notation" constr(f) := change f with (`f).
 Tactic Notation "fold" "notation" constr(f) := unfold make_visible.
 
 Definition bv_eqb {n} (x y : bv n) : bool :=
-  Eval cbv beta iota zeta delta [ bool_decide decide_rel ] in
+  Eval cbv delta [ bool_decide decide_rel ] in
     bool_decide (x = y).
 
 Definition bv_odd {n} (x : bv n) := Z.odd (bv_unsigned x).
@@ -54,6 +54,8 @@ Infix "#" := bv_zero_extend (at level 65) : bv_scope.
 Infix "||" := (bv_concat _) : bv_scope.
 
 Notation "x ?" := (bv_odd x) : bv_scope.
+
+(**********************************************************************************)
 
 Record Registers :=
   mkRegisters { r_A : bv 8 ; r_B : bv 4 ; r_cnt : bv 2 ; r_busy : bv 1}.
@@ -132,222 +134,221 @@ Fixpoint cycles (s : State) (xs : list In) : State * list Out :=
       (s'', y :: ys)
   end.
 
-Fixpoint cycles' (s : State) (xs : list In) : State :=
-  match xs with
-  | [] => s
-  | x :: xs' => cycles' (fst (cycle s x)) xs'
-  end.
+Definition cycle' s x := fst (cycle s x).
 
-Fixpoint repeat {A : Type} (f : A -> A) (n : nat) {struct n} : (A -> A) :=
-  match n with
-  | O => id
-  | S n' => f ∘ repeat f n'
-  end.
+Definition cycles' s xs := fold_left cycle' xs s.
 
-Definition repeat_shift_and_add n b a := (repeat (shift_and_add b) n) a.
-
-Definition shift_and_add4 := repeat_shift_and_add 4.
-
-Definition shift_and_add' (b a : Z) :=
-  Z.lor (bv_wrap 5 (a ≫ 4 + (bv_wrap 1 a * b)) ≪ 3) (bv_wrap 3 (a ≫ 1)).
-
-Definition repeat_shift_and_add' n b a := (repeat (shift_and_add' b) n) a.
-
-Definition shift_and_add4' := repeat_shift_and_add' 4.
-
-Lemma shift_and_add_equiv : forall a b,
-    shift_and_add' (bv_unsigned b) (bv_unsigned a) =
-      bv_unsigned (shift_and_add b a).
-Proof.
-  intros a b. unfold shift_and_add, shift_and_add'. bv_simplify.
-  unfold Z.of_N, bv_odd. unfold notation Z.modulo. Search (_ `mod` 2)%Z.
-  unfold bv_wrap. rewrite Zmod_odd. case_match.
-  - replace (1 * bv_unsigned b)%Z with (bv_unsigned b) by lia. bv_solve.
-  - Search (0 * _)%Z. rewrite Z.mul_0_l. bv_solve.
-Qed.
-
-Lemma shift_and_add_repeat_equiv : forall n a b,
-    (repeat_shift_and_add' n) (bv_unsigned b) (bv_unsigned a) =
-      bv_unsigned (repeat_shift_and_add n b a).
-Proof.
-  intros n a b. induction n; simplify.
-  - unfold repeat_shift_and_add', repeat_shift_and_add. done.
-  - unfold repeat_shift_and_add', repeat_shift_and_add in *. simplify.
-    rewrite IHn. apply shift_and_add_equiv.
-Qed.
-
-Lemma shift_and_add4_equiv : forall a b,
-    shift_and_add4' (bv_unsigned b) (bv_unsigned a) =
-      bv_unsigned (shift_and_add4 b a).
-Proof.
-  unfold shift_and_add4', shift_and_add4. apply shift_and_add_repeat_equiv.
-Qed.
-
-(* Tactic for exhaustive case analysis on integers in range [0,16) *)
-(* Automatically finds variables with range hypotheses and does case analysis *)
-Ltac by_cases16 :=
-  repeat match goal with
-    | [ H : (0 <= ?z < 16)%Z |- _ ] =>
-        let Hz := fresh "Hcases" in
-        assert (z = 0 \/ z = 1 \/ z = 2 \/ z = 3 \/ z = 4 \/ z = 5 \/ z = 6 \/ z = 7 \/
-                  z = 8 \/ z = 9 \/ z = 10 \/ z = 11 \/ z = 12 \/ z = 13 \/ z = 14 \/ z = 15)%Z
-          as Hz by lia; clear H;
-        destruct_or?; subst
-    end; done.
-
-Lemma shift_and_add4'_multiplies : forall a b,
-    (0 <= a < bv_modulus 4%N)%Z ->
-    (0 <= b < bv_modulus 4%N)%Z ->
-    shift_and_add4' b a = (a * b)%Z.
-Proof.
-  intros a b Ha Hb. replace (bv_modulus 4%N) with 16%Z in * by easy. by_cases16.
-Qed.
-
-Lemma shift_and_add4_multiplies : forall (a b : bv 4),
-    bv_unsigned (shift_and_add4 b (8#a)) = (bv_unsigned a * bv_unsigned b)%Z.
-Proof.
-  intros a b. rewrite <- shift_and_add4_equiv.
-  Search bv_unsigned bv_zero_extend. rewrite bv_zero_extend_unsigned by lia.
-  apply shift_and_add4'_multiplies. all: bv_solve.
-Qed.
-
-Notation "a *| b" := ((8#a) * (8#b)) (at level 35).
-
-Lemma shift_and_add4_correct : forall (a b : bv 4),
-    shift_and_add4 b (8#a) = a *| b.
-Proof.
-  intros a b. Search (bv_unsigned _ = bv_unsigned _).
-  rewrite bv_eq. Search bv_mul.
-  rewrite bv_mul_unsigned.
-  Search bv_zero_extend bv_unsigned.
-  repeat rewrite bv_zero_extend_unsigned by lia.
-  Check bv_wrap_small. rewrite bv_wrap_small.
-  apply shift_and_add4_multiplies. bv_saturate_unsigned.
-  unfold bv_modulus in *; simplify. nia.
-Qed.
-
-Lemma bv1_is_0_or_1 : forall (b : bv 1), b = 0 \/ b = 1.
-Proof.
-  intro b. Search "bv" "ind".
-  apply bv_1_ind with (P := (fun b => b = 0 \/ b = 1)); intuition congruence.
-Qed.
-
-Definition busy (s : State) := s.(R).(r_busy) = 1.
-Definition finished (s : State) := s.(R).(r_cnt) = 0.
-Definition valid (x : In) := x.(in_valid) = 1.
-
-Hint Extern 1 (_ = _ :> bv 1) =>
-       match goal with
-       | |- ?b = 0 :> bv 1 => pose proof (bv1_is_0_or_1 b); intuition
-       | |- ?b = 1 :> bv 1 => pose proof (bv1_is_0_or_1 b); intuition
-       end : multiplier.
-
-Definition cycle_idle_valid s1 x s2 y : Prop :=
-  ~ busy s1 -> valid x -> (s2, y) = cycle s1 x ->
-  (s2, y) = (s1 <| R := {| r_A := 8#x.(in_A); r_B := x.(in_B); r_cnt := 3; r_busy := 1 |} |>
-                <| T := s1.(T) ++ [{| leak_valid := 1; leak_ready := 0 |}] |>,
-             Out0).
-
-Lemma cycle_idle_valid_holds : forall s1 x s2 y, cycle_idle_valid s1 x s2 y.
-Proof.
-  unfold cycle_idle_valid. simplify.
-  unfold cycle in *. unfold bv_eqb in *. unfold busy in *.
-  unfold valid in *. assert (s1.(R).(r_busy) = 0) by auto with multiplier.
-  repeat rewrite H2 in H1. simpl in *. rewrite H0 in H1.
-  simplify. inv H1. done.
-Qed.
-
-Definition cycle_idle_invalid s1 x s2 y : Prop :=
-  ~ busy s1 -> ~ valid x -> (s2, y) = cycle s1 x ->
-  (s2, y) = (s1 <| T := s1.(T) ++ [{| leak_valid := 0; leak_ready := 0 |}] |>,
-             Out0).
-
-Lemma cycle_idle_invalid_holds : forall s1 x s2 y, cycle_idle_invalid s1 x s2 y.
-Proof.
-  unfold cycle_idle_invalid. simplify.
-  unfold cycle, bv_eqb, busy, valid in *.
-  assert (s1.(R).(r_busy) = 0) by auto with multiplier.
-  assert (x.(in_valid) = 0) by auto with multiplier.
-  rewrite H2, H3 in H1. simpl in *. inversion H1; clear H1.
-  done.
-Qed.
-
-Definition cycle_busy_unfinished s1 x s2 y : Prop :=
-  busy s1 -> ~ finished s1 -> (s2, y) = cycle s1 x ->
-  (s2, y) = (s1 <| R; r_A := shift_and_add s1.(R).(r_B) s1.(R).(r_A) |>
-                <| R; r_cnt := s1.(R).(r_cnt) - 1 |>
-                <| T := s1.(T) ++ [{| leak_valid := x.(in_valid); leak_ready := 0 |}] |>,
-              Out0).
-
-Lemma cycle_busy_unfinished_holds : forall s1 x s2 y, cycle_busy_unfinished s1 x s2 y.
-Proof.
-  unfold cycle_busy_unfinished. simplify.
-  unfold cycle, bv_eqb, busy, finished in *.
-  rewrite H in H1; simpl in *.
-  destruct (bv_eq_dec 2 (r_cnt (R s1)) 0) as [Heq | Hneq].
-  - done.
-  - inv H1. intuition congruence.
-Qed.
-
-Definition cycle_busy_finished s1 x s2 y : Prop :=
-  busy s1 -> finished s1 -> (s2, y) = cycle s1 x ->
-  (s2, y) = (s1 <| R; r_A := shift_and_add s1.(R).(r_B) s1.(R).(r_A) |>
-                <| R; r_cnt := 0 |>
-                <| R; r_busy := 0 |>
-                <| T := s1.(T) ++ [{| leak_valid := x.(in_valid); leak_ready := 1 |}] |>,
-                {| out_P := s2.(R).(r_A); out_ready := 1 |}).
-
-Lemma cycle_busy_finished_holds : forall s1 x s2 y, cycle_busy_finished s1 x s2 y.
-Proof.
-  unfold cycle_busy_finished. simplify.
-  unfold cycle, bv_eqb, busy, finished in *.
-  rewrite H in H1; simplify. rewrite H0 in H1.
-  simplify. inversion H1; clear H1; subst. done.
-Qed.
-
-Ltac unfold_cycle_predicates :=
-  unfold cycle_idle_valid, cycle_idle_invalid, cycle_busy_unfinished,
-    cycle_busy_finished, busy, finished, valid in *.
-
-Ltac unfold_pair H := inversion H; clear H.
-
-Ltac unfold_pairs :=
-  repeat match goal with
-    | H : (_, _) = (_, _) |- _ => unfold_pair H
+Section functional.
+  Fixpoint repeat {A : Type} (f : A -> A) (n : nat) {struct n} : (A -> A) :=
+    match n with
+    | O => id
+    | S n' => f ∘ repeat f n'
     end.
 
-Ltac unroll_let e :=
-  let Hlet := fresh "Hlet0" in destruct e eqn:Hlet; symmetry in Hlet.
+  Definition repeat_shift_and_add n b a := (repeat (shift_and_add b) n) a.
 
-Ltac unroll_lets :=
-  repeat match goal with
-    | [ H : context[let (_, _) := (cycle ?x ?y) in _] |- _ ] =>
-        unroll_let (cycle x y)
-    end.
+  Definition shift_and_add4 := repeat_shift_and_add 4.
 
-Ltac cycles_correct_auto :=
-  unfold_pairs; subst; try (unfold_cycle_predicates; solve
-                        [ intuition
-                        | simplify; bv_solve ]).
+  Definition shift_and_add' (b a : Z) :=
+    Z.lor (bv_wrap 5 (a ≫ 4 + (bv_wrap 1 a * b)) ≪ 3) (bv_wrap 3 (a ≫ 1)).
 
-(* Finally, with all those helper theorems out of the way, we can now prove the
-   following correctness property:
+  Definition repeat_shift_and_add' n b a := (repeat (shift_and_add' b) n) a.
 
-   For any cycle where the circuit is idle, if a valid [a] and [b] are provided,
-   four cycles later it will produce [a *| b]. *)
-Theorem cycles_correct : forall s s' x1 x2 x3 x4 x5 ys a b,
-    ~ busy s -> x1 = {| in_A := a; in_B := b; in_valid := 1 |} ->
-    (s', ys) = cycles s [x1; x2; x3; x4; x5] ->
-    ys = [Out0; Out0; Out0; Out0; {| out_P := a *| b; out_ready := 1 |}].
-Proof.
-  simplify. unroll_lets.
-  apply cycle_idle_valid_holds      in Hlet0; cycles_correct_auto.
-  apply cycle_busy_unfinished_holds in Hlet1; cycles_correct_auto.
-  apply cycle_busy_unfinished_holds in Hlet2; cycles_correct_auto.
-  apply cycle_busy_unfinished_holds in Hlet3; cycles_correct_auto.
-  apply cycle_busy_finished_holds   in Hlet4; cycles_correct_auto.
-  simplify. repeat f_equal. by apply shift_and_add4_correct.
-Qed.
+  Definition shift_and_add4' := repeat_shift_and_add' 4.
+
+  Lemma shift_and_add_equiv : forall a b,
+      shift_and_add' (bv_unsigned b) (bv_unsigned a) =
+        bv_unsigned (shift_and_add b a).
+  Proof.
+    intros a b. unfold shift_and_add, shift_and_add'. bv_simplify.
+    unfold Z.of_N, bv_odd. unfold notation Z.modulo. Search (_ `mod` 2)%Z.
+    unfold bv_wrap. rewrite Zmod_odd. case_match.
+    - replace (1 * bv_unsigned b)%Z with (bv_unsigned b) by lia. bv_solve.
+    - Search (0 * _)%Z. rewrite Z.mul_0_l. bv_solve.
+  Qed.
+
+  Lemma shift_and_add_repeat_equiv : forall n a b,
+      (repeat_shift_and_add' n) (bv_unsigned b) (bv_unsigned a) =
+        bv_unsigned (repeat_shift_and_add n b a).
+  Proof.
+    intros n a b. induction n; simplify.
+    - unfold repeat_shift_and_add', repeat_shift_and_add. done.
+    - unfold repeat_shift_and_add', repeat_shift_and_add in *. simplify.
+      rewrite IHn. apply shift_and_add_equiv.
+  Qed.
+
+  Lemma shift_and_add4_equiv : forall a b,
+      shift_and_add4' (bv_unsigned b) (bv_unsigned a) =
+        bv_unsigned (shift_and_add4 b a).
+  Proof.
+    unfold shift_and_add4', shift_and_add4. apply shift_and_add_repeat_equiv.
+  Qed.
+
+  (* Tactic for exhaustive case analysis on integers in range [0,16) *)
+  (* Automatically finds variables with range hypotheses and does case analysis *)
+  Ltac by_cases16 :=
+    repeat match goal with
+      | [ H : (0 <= ?z < 16)%Z |- _ ] =>
+          let Hz := fresh "Hcases" in
+          assert (z = 0 \/ z = 1 \/ z = 2 \/ z = 3 \/ z = 4 \/ z = 5 \/ z = 6 \/ z = 7 \/
+                    z = 8 \/ z = 9 \/ z = 10 \/ z = 11 \/ z = 12 \/ z = 13 \/ z = 14 \/ z = 15)%Z
+            as Hz by lia; clear H;
+          destruct_or?; subst
+      end; done.
+
+  Lemma shift_and_add4'_multiplies : forall a b,
+      (0 <= a < bv_modulus 4%N)%Z ->
+      (0 <= b < bv_modulus 4%N)%Z ->
+      shift_and_add4' b a = (a * b)%Z.
+  Proof.
+    intros a b Ha Hb. replace (bv_modulus 4%N) with 16%Z in * by easy. by_cases16.
+  Qed.
+
+  Lemma shift_and_add4_multiplies : forall (a b : bv 4),
+      bv_unsigned (shift_and_add4 b (8#a)) = (bv_unsigned a * bv_unsigned b)%Z.
+  Proof.
+    intros a b. rewrite <- shift_and_add4_equiv.
+    Search bv_unsigned bv_zero_extend. rewrite bv_zero_extend_unsigned by lia.
+    apply shift_and_add4'_multiplies. all: bv_solve.
+  Qed.
+
+  Notation "a *| b" := ((8#a) * (8#b)) (at level 35).
+
+  Lemma shift_and_add4_correct : forall (a b : bv 4),
+      shift_and_add4 b (8#a) = a *| b.
+  Proof.
+    intros a b. Search (bv_unsigned _ = bv_unsigned _).
+    rewrite bv_eq. Search bv_mul.
+    rewrite bv_mul_unsigned.
+    Search bv_zero_extend bv_unsigned.
+    repeat rewrite bv_zero_extend_unsigned by lia.
+    Check bv_wrap_small. rewrite bv_wrap_small.
+    apply shift_and_add4_multiplies. bv_saturate_unsigned.
+    unfold bv_modulus in *; simplify. nia.
+  Qed.
+
+  Lemma bv1_is_0_or_1 : forall (b : bv 1), b = 0 \/ b = 1.
+  Proof.
+    intro b. Search "bv" "ind".
+    apply bv_1_ind with (P := (fun b => b = 0 \/ b = 1)); intuition congruence.
+  Qed.
+
+  Definition busy (s : State) := s.(R).(r_busy) = 1.
+  Definition finished (s : State) := s.(R).(r_cnt) = 0.
+  Definition valid (x : In) := x.(in_valid) = 1.
+
+  Hint Extern 1 (_ = _ :> bv 1) =>
+         match goal with
+         | |- ?b = 0 :> bv 1 => pose proof (bv1_is_0_or_1 b); intuition
+| |- ?b = 1 :> bv 1 => pose proof (bv1_is_0_or_1 b); intuition
+  end : multiplier.
+
+  Definition cycle_idle_valid s1 x s2 y : Prop :=
+    ~ busy s1 -> valid x -> (s2, y) = cycle s1 x ->
+    (s2, y) = (s1 <| R := {| r_A := 8#x.(in_A); r_B := x.(in_B); r_cnt := 3; r_busy := 1 |} |>
+                  <| T := s1.(T) ++ [{| leak_valid := 1; leak_ready := 0 |}] |>,
+               Out0).
+
+  Lemma cycle_idle_valid_holds : forall s1 x s2 y, cycle_idle_valid s1 x s2 y.
+  Proof.
+    unfold cycle_idle_valid. simplify.
+    unfold cycle in *. unfold bv_eqb in *. unfold busy in *.
+    unfold valid in *. assert (s1.(R).(r_busy) = 0) by auto with multiplier.
+    repeat rewrite H2 in H1. simplify. rewrite H0 in H1.
+    simplify. inv H1. done.
+  Qed.
+
+  Definition cycle_idle_invalid s1 x s2 y : Prop :=
+    ~ busy s1 -> ~ valid x -> (s2, y) = cycle s1 x ->
+    (s2, y) = (s1 <| T := s1.(T) ++ [{| leak_valid := 0; leak_ready := 0 |}] |>,
+               Out0).
+
+  Lemma cycle_idle_invalid_holds : forall s1 x s2 y, cycle_idle_invalid s1 x s2 y.
+  Proof.
+    unfold cycle_idle_invalid. simplify.
+    unfold cycle, bv_eqb, busy, valid in *.
+    assert (s1.(R).(r_busy) = 0) by auto with multiplier.
+    assert (x.(in_valid) = 0) by auto with multiplier.
+    rewrite H2, H3 in H1. simplify. inv H1. done.
+  Qed.
+
+  Definition cycle_busy_unfinished s1 x s2 y : Prop :=
+    busy s1 -> ~ finished s1 -> (s2, y) = cycle s1 x ->
+    (s2, y) = (s1 <| R; r_A := shift_and_add s1.(R).(r_B) s1.(R).(r_A) |>
+                  <| R; r_cnt := s1.(R).(r_cnt) - 1 |>
+                  <| T := s1.(T) ++ [{| leak_valid := x.(in_valid); leak_ready := 0 |}] |>,
+               Out0).
+
+  Lemma cycle_busy_unfinished_holds : forall s1 x s2 y, cycle_busy_unfinished s1 x s2 y.
+  Proof.
+    unfold cycle_busy_unfinished. simplify.
+    unfold cycle, bv_eqb, busy, finished in *.
+    rewrite H in H1; simplify.
+    destruct (bv_eq_dec 2 (r_cnt (R s1)) 0) as [Heq | Hneq].
+    - done.
+    - inv H1. intuition congruence.
+  Qed.
+
+  Definition cycle_busy_finished s1 x s2 y : Prop :=
+    busy s1 -> finished s1 -> (s2, y) = cycle s1 x ->
+    (s2, y) = (s1 <| R; r_A := shift_and_add s1.(R).(r_B) s1.(R).(r_A) |>
+                  <| R; r_cnt := 0 |>
+                  <| R; r_busy := 0 |>
+                  <| T := s1.(T) ++ [{| leak_valid := x.(in_valid); leak_ready := 1 |}] |>,
+                  {| out_P := s2.(R).(r_A); out_ready := 1 |}).
+
+  Lemma cycle_busy_finished_holds : forall s1 x s2 y, cycle_busy_finished s1 x s2 y.
+  Proof.
+    unfold cycle_busy_finished. simplify.
+    unfold cycle, bv_eqb, busy, finished in *.
+    rewrite H in H1; simplify. rewrite H0 in H1.
+    simplify. inv H1. done.
+  Qed.
+
+  Ltac unroll_cycle_predicates :=
+    unfold cycle_idle_valid, cycle_idle_invalid, cycle_busy_unfinished,
+      cycle_busy_finished, busy, finished, valid in *.
+
+  Ltac unfold_pair H := inversion H; clear H.
+
+  Ltac unfold_pairs :=
+    repeat match goal with
+      | H : (_, _) = (_, _) |- _ => unfold_pair H
+      end.
+
+  Ltac unroll_let e :=
+    let Hlet := fresh "Hlet0" in destruct e eqn:Hlet; symmetry in Hlet.
+
+  Ltac unroll_lets :=
+    repeat match goal with
+      | [ H : context[let (_, _) := (cycle ?x ?y) in _] |- _ ] =>
+          unroll_let (cycle x y)
+      end.
+
+  Ltac cycles_correct_auto :=
+    unfold_pairs; subst; try (unroll_cycle_predicates; solve
+                                                         [ intuition
+                                                         | simplify; bv_solve ]).
+
+  (* Finally, with all those helper theorems out of the way, we can now prove
+     the following correctness property:
+
+     For any cycle where the circuit is idle, if a valid [a] and [b] are
+     provided, four cycles later it will produce [a *| b]. *)
+  Theorem cycles_correct : forall s s' x1 x2 x3 x4 x5 ys a b,
+      ~ busy s -> x1 = {| in_A := a; in_B := b; in_valid := 1 |} ->
+      (s', ys) = cycles s [x1; x2; x3; x4; x5] ->
+      ys = [Out0; Out0; Out0; Out0; {| out_P := a *| b; out_ready := 1 |}].
+  Proof.
+    simplify. unroll_lets.
+    apply cycle_idle_valid_holds      in Hlet0; cycles_correct_auto.
+    apply cycle_busy_unfinished_holds in Hlet1; cycles_correct_auto.
+    apply cycle_busy_unfinished_holds in Hlet2; cycles_correct_auto.
+    apply cycle_busy_unfinished_holds in Hlet3; cycles_correct_auto.
+    apply cycle_busy_finished_holds   in Hlet4; cycles_correct_auto.
+    simplify. repeat progress f_equal. by apply shift_and_add4_correct.
+  Qed.
+End functional.
 
 (* NOTE knwabueze for aerbsen: I think we talked about using this definition for
    the extraction from the list of inputs to the specification leakage.
@@ -361,64 +362,109 @@ Qed.
     function would need to know whether or not a value for [A] was provided on
     each cycle, not just the total list of provided values. *)
 
-Definition SLeakage := option (bv 4).
+Section ct.
+  Definition SLeakage := option (bv 4).
 
-Definition extract : list In -> list SLeakage :=
-  map (fun x => if x.(in_valid) =? 1 then Some x.(in_A) else None).
+  Definition extract x := if x.(in_valid) =? 1 then Some x.(in_A) else None.
 
-(* Predictor function which uses the prefix of the specification leakage trace
-   to predict the next item in the implementation leakage trace. *)
-Definition update_st (st : option nat * bool) (s : SLeakage) :=
-  match st with
-  | (Some (S n), _) =>
-      match s with
-      | Some _ => (Some n, true)
-      | None => (Some n, false)
-      end
-  | (Some O, _) =>
-      match s with
-      | Some _ => (None, true)
-      | None => (None, false)
-      end
-  | (None, _) =>
-      match s with
-      | Some _ => (Some 4%nat, true)
-      | None => (None, false)
-      end
-  end.
+  Definition extract_many : list In -> list SLeakage := map extract.
 
-Fixpoint predict_next' (prefix : list SLeakage) (st : option nat * bool) : ILeakage :=
-  match prefix with
-  | [] =>
-      match st with
-      | (None  , v) => {| leak_valid := bool_to_bv 1 v; leak_ready := 0 |}
-      | (Some O, v) => {| leak_valid := bool_to_bv 1 v; leak_ready := 1 |}
-      | (Some _, v) => {| leak_valid := bool_to_bv 1 v; leak_ready := 0 |}
-      end
-  | p :: ps => predict_next' ps (update_st st p)
-  end.
+  (* Predictor function uses the prefix of the specification leakage trace to
+     predict the next item in the implementation leakage trace.
 
-Definition predict_next prefix := predict_next' prefix (None, false).
+     The predictor can be seen as a state machine with some simulation relation
+     [R] to our circuit. *)
 
-Fixpoint predict' prefix xs :=
-  match xs with
-  | [] => []
-  | x :: xs' => predict_next (prefix ++ [x]) :: predict' (prefix ++ [x]) xs'
-  end.
+  Record PredictorState :=
+    mkPredictorState { ps_count : option nat ; ps_valid : bool }.
 
-Definition predict xs := predict' [] xs.
+  Definition PredictorState0 := mkPredictorState None false.
 
-(* First, we need a helper lemma that talks about one cycle's behavior on a the
-   implementation leakage trace. This follows by doing cases analysis on the
-   four fundamental outcomes that may happen on a cycle:
+  Definition predictor_step (st : PredictorState) (s : SLeakage) :=
+    match st with
+    | {| ps_count := Some (S n) |} =>
+        match s with
+        | Some _ => {| ps_count := Some n; ps_valid := true |}
+        | None   => {| ps_count := Some n; ps_valid := false |}
+        end
+    | {| ps_count := Some O |} =>
+        match s with
+        | Some _ => {| ps_count := None; ps_valid := true |}
+        | None   => {| ps_count := None; ps_valid := false |}
+        end
+    | {| ps_count := None |} =>
+        match s with
+        | Some _ => {| ps_count := Some 4%nat; ps_valid := true |}
+        | None   => {| ps_count := None; ps_valid := false |}
+        end
+    end.
 
-   1. The circuit is idle and recieves an invalid input.
-   2. The circuit is idle and recieves a valid input.
-   3. The circuit is busy, but r_cnt > 0.
-   4. The circuit is busy, but r_cnt = 0. *)
+  Definition predictor_steps (st : PredictorState) (ss : list SLeakage) :=
+    fold_left predictor_step ss st.
 
-Theorem cycles_ct : exists f, forall xs ys s,
-    ys = extract xs ->
-    s = cycles' State0 xs ->
-    s.(T) = f ys.
-Admitted.
+  Definition predict_next prefix :=
+    match predictor_steps PredictorState0 prefix with
+    | {| ps_count := Some (S _); ps_valid := v |} =>
+        {| leak_valid := bool_to_bv 1 v; leak_ready := 0 |}
+    | {| ps_count := Some O; ps_valid := v |} =>
+        {| leak_valid := bool_to_bv 1 v; leak_ready := 1 |}
+    | {| ps_count := None; ps_valid := v |} =>
+        {| leak_valid := bool_to_bv 1 v; leak_ready := 0 |}
+    end.
+
+  Fixpoint predict' prefix xs :=
+    match xs with
+    | [] => []
+    | x :: xs' => predict_next (prefix ++ [x]) :: predict' (prefix ++ [x]) xs'
+    end.
+
+  Definition predict xs := predict' [] xs.
+
+  Lemma predict_continuity' : forall ys y t t' p,
+      t = predict' p ys ->
+      t' = predict' p (ys ++ [y]) ->
+      t' = t ++ [predict_next (p ++ ys ++ [y])].
+  Proof.
+    induction ys as [| y' ys']; simplify.
+    - done.
+    - f_equal.
+      replace (p ++ y' :: ys' ++ [y]) with (p ++ [y'] ++ ys' ++ [y]); cycle 1.
+      { Search (_ ++ _ :: _ = _ ++ [_] ++ _). rewrite <- cons_middle. done. }
+      specialize (IHys' y
+                    (predict' (p ++ [y']) ys')
+                    (predict' (p ++ [y']) (ys' ++ [y]))
+                    (p ++ [y'])).
+      rewrite app_assoc. apply IHys'; done.
+  Qed.
+
+  Corollary predict_continuity : forall ys y t t',
+      t = predict ys ->
+      t' = predict (ys ++ [y]) ->
+      t' = t ++ [predict_next (ys ++ [y])].
+  Proof.
+    unfold predict; intros.
+    Search ([] ++ _ = _).
+    replace ys with ([] ++ ys) by apply app_nil_l.
+    rewrite <- app_assoc.
+    apply predict_continuity'; done.
+  Qed.
+
+  Lemma cycles_continuity' : forall ,
+      s' = cycles' s xs ->
+      s'' = cycle' s' x ->
+      s''.(T) = s'.(T)
+
+  (* First, we need a helper lemma that talks about one cycle's behavior on a the
+     implementation leakage trace. This follows by doing cases analysis on the
+     four fundamental outcomes that may happen on a cycle:
+
+     1. The circuit is idle and recieves an invalid input.
+     2. The circuit is idle and recieves a valid input.
+     3. The circuit is busy, but r_cnt > 0.
+     4. The circuit is busy, but r_cnt = 0. *)
+  Theorem cycles_ct : exists f, forall xs ys s,
+      ys = extract_many xs ->
+      s = cycles' State0 xs ->
+      s.(T) = f ys.
+  Admitted.
+End ct.
